wip

theories/check_ho.v
@@ -1,30 +1,215 @@
 From det Require Import prelude.
 From mathcomp Require Import all_ssreflect.
-From det Require Import tree tree_prop ctx tree_vars unif mut_excl fresh.
+From det Require Import tree tree_prop ctx tree_vars unif mut_excl fresh sig_lattice compat_sig.
+From elpi.apps Require Import derive derive.std.
+From HB Require Import structures.
+
+Definition sigV := {fmap V -> S}.
+
+Definition is_sigV (x : sigV) := unit.
+Lemma is_sigV_inhab : forall x, is_sigV x. Proof. exact (fun x => tt). Qed.
+Definition sigV_eqb (x y : sigV) := x == y.
+Lemma sigV_eqb_correct : forall x, eqb_correct_on sigV_eqb x. Proof. by move=>??/eqP. Qed.
+Lemma sigV_eqb_refl : forall x, eqb_refl_on sigV_eqb x. Proof. by move=>?; exact: eqxx. Qed.
+Elpi derive.eqbOK.register_axiomx sigV is_sigV is_sigV_inhab sigV_eqb sigV_eqb_correct sigV_eqb_refl.
+HB.instance Definition _ : hasDecEq sigV := Equality.copy sigV _.
 
 Section checker.
 
-  Definition check_atom sP (a: Atom) :=
+  Definition odflt1 {T} (ab : T * bool) x := 
+    match x with (Some x, b1) => (x,b1) | (None,_) => ab end.
+
+  Definition flex_head T := if get_tm_hd T is inr (inr _) then true else false.
+
+  (* takes a tm and a signature and updates variable signatures
+     updates are performed only on variables in input positions *)
+  (* Invariant: length s = length t *)
+  Fixpoint assume_tm (sP:sigT) (sV:sigV) (tm : seq Tm) (s : seq mode) (t: seq S): sigV :=
+    match s, t, tm with
+    | _, _, [::] | [::], _, _ | _, [::], _ => sV
+    | output :: ms, _  :: tys, _ :: ts => assume_tm sP sV ts ms tys
+    | input  :: ms, ty :: tys, t :: ts =>
+      let sV := match t with
+      | Tm_V v =>
+        match sV.[? v] with
+        | None => sV.[v <- ty]
+        | Some oldv =>
+          if compat_type oldv ty then add v (min ty oldv) sV else sV
+        end
+      | _ => sV end in  (*TODO: complete this pattern*)
+      assume_tm sP sV ts ms tys
+    end.
+
+  (* returns the signature of the term and if it is well called *)
+  Fixpoint check_tm (sP:sigT) (sV:sigV) (tm : Tm)  : S * bool :=
+    match tm with
+    | Tm_D k => (b Exp, true)
+    | Tm_P k => odflt1 (b(d Pred),false) (lookup k sP, true)
+    | Tm_V v =>  odflt1 (b(d Pred),false) (lookup v sV, true)
+    | Tm_App l r => 
+        (* before we check the LHS and then we go right *)
+        let (sl, b1) := check_tm sP sV l  in
+        (* if the type of l is not an arrow, we return anyT *)
+        if sl is arr m tl tr then
+          if m == input then
+            let (cr, br) := check_tm sP sV r in
+            if incl cr tl && b1 && br then (tr, true)
+            else (weak tr, false)
+          else (tr, b1)
+        else (b(d Pred),false)
+    end.
+
+  (* Definition subst2sig sP (s: Sigma) :=
+    let x := [fmap x: domf s => check_tm sP empty s.[valP x]] in
+    fmap_filter. *)
+
+
+  (* returns the determinacy of the term t *)
+  Definition call_is_det sP sV t :=
+    check_tm sP sV t == (b (d Func), true).
+
+  (* Fixpoint check_atoms sP sV s d :=
+    match s with
+    | [::] => d
+    | cut :: xs => check_atoms sP sV xs Func
+    | call t :: xs => check_atoms sP sV xs (maxD d (call_is_det sP sV t))
+    end. *)
+
+  Definition check_atom sP sV (a: Atom) :=
     match a with
     | cut => true
-    | call t => tm_is_det sP t
+    | call t => call_is_det sP sV t
     end. 
 
   (* There is cut and after the cut there are only call to Det preds *)
-  Fixpoint check_atoms (sP :sigT) (s: seq Atom) :=
+  Fixpoint check_atoms (sP :sigT) sV (s: seq Atom) :=
     match s with
     | [::] => true
-    | cut :: xs => all (check_atom sP) xs || check_atoms sP xs
-    | call c :: xs => (tm_is_det sP c || has_cut_seq xs) && check_atoms sP xs
+    | cut :: xs => all (check_atom sP sV) xs || check_atoms sP sV xs
+    | call c :: xs => (call_is_det sP sV c || has_cut_seq xs) && check_atoms sP sV xs
     end.
-
-  Definition check_rule sP head prems :=
-    (tm_is_det sP head == false) || 
-      check_atoms sP prems.
+    
+  Definition check_rule (sP:sigT) head prems :=
+    match get_tm_hd head with
+    | inl pred =>
+      if sP.[? pred] is Some sig then
+        let md := flatten_mode sig in
+        let tys := flatten_sig sig in
+        let args := flatten_term head in
+        let sV := assume_tm sP empty args md tys in
+        (tm_is_det sP head == false) || 
+          (check_atoms sP sV prems)
+      else true
+    | _ => true
+    end.
 
   Definition check_rules p :=
     all (fun x => check_rule p.(sig) x.(head) x.(premises)) p.(rules).
 End checker.
+
+
+Module Test.
+  Definition p := b (d Pred).
+  Definition f := b (d Func).
+  Definition e := b Exp.
+  Notation V1 := (IV 0).
+  Notation V2 := (IV 1).
+  Notation F := (IV 2).
+  
+  Definition mkP sym sig r := {| sig := [fmap].[sym <- sig]; rules := [::r] |}.
+
+  Module Once.
+    Notation onceSym := (IP 1).
+    Definition onceI   := mkR (Tm_App (Tm_P onceSym) (Tm_V V1)) [::call (Tm_V V1); cut].
+    Definition onceSig := arr input p f.
+
+    Goal check_rules (mkP onceSym onceSig onceI).
+    Proof.
+      rewrite/check_rules/=andbT/check_rule.
+      rewrite [get_tm_hd _]/=.
+      cbn match.
+      rewrite in_fnd; first by rewrite !in_fsetE eqxx.
+      move=> H.
+      rewrite/tm_is_det [get_tm_hd _]/=.
+      cbn match.
+      rewrite !FmapE.fmapE orFb.
+      by case: eqP => //=; rewrite not_fnd//= /call_is_det /check_tm !FmapE.fmapE/=.
+    Qed.
+  End Once.
+  
+  Module Do.
+    Notation doSym := (IP 2).
+    Definition doI   := mkR (Tm_App (Tm_P doSym) (Tm_V V1)) [::call (Tm_V V1)].
+    Definition doSig := arr input f f.
+
+    Goal check_rules (mkP doSym doSig doI).
+    Proof.
+      rewrite/check_rules/=andbT/check_rule.
+      rewrite [get_tm_hd _]/=.
+      cbn match.
+      rewrite in_fnd; first by rewrite !in_fsetE eqxx.
+      move=> H.
+      rewrite/tm_is_det [get_tm_hd _]/=.
+      cbn match.
+      rewrite !FmapE.fmapE not_fnd//.
+      rewrite [flatten_term _]/= [flatten_mode _]/= [flatten_sig _]/=.
+      case:eqP => // _.
+      rewrite orFb.
+      rewrite [flatten_mode _]/= [flatten_sig _]/=.
+      rewrite/assume_tm not_fnd//.
+      rewrite/check_atoms /tm_is_det.
+      rewrite/call_is_det /check_tm.
+      by rewrite FmapE.fmapE/=.
+    Qed.
+  End Do.
+  
+  (* apply F X :- F X. *)
+  Module Apply.
+    Notation applySym := (IP 3).
+    Definition applyI   := mkR (Tm_App (Tm_App (Tm_P applySym) (Tm_V F)) (Tm_V V1)) [::call (Tm_App (Tm_V F) (Tm_V V1))].
+    Definition applySig := arr input (arr input e f) (arr input e f).
+
+    Goal check_rules (mkP applySym applySig applyI).
+    Proof.
+      rewrite/check_rules/= andbT/check_rule.
+      rewrite [get_tm_hd _]/=.
+      cbn match.
+      rewrite !FmapE.fmapE eqxx .
+      rewrite [flatten_term _]/= [flatten_mode _]/= [flatten_sig _]/=.
+      rewrite/tm_is_det/get_tm_hd FmapE.fmapE.
+      rewrite orFb.
+      (* assume head *)
+      rewrite/assume_tm (@not_fnd _ _ _ (IV 2))//.
+      rewrite !FmapE.fmapE not_fnd//=.
+      (* check body, with F: exp -> func, and V1: e *)
+      by rewrite/call_is_det /check_tm !FmapE.fmapE eqxx.
+    Qed.
+  End Apply.
+  
+  (* apply F X :- F X. *)
+  Module WrongApply.
+    Notation applySym := (IP 3).
+    Definition applyI   := mkR (Tm_App (Tm_App (Tm_P applySym) (Tm_V F)) (Tm_V V1)) [::call (Tm_App (Tm_V F) (Tm_V V1))].
+    Definition applySig := arr input (arr input e p) (arr input e f).
+
+    Goal ~~ check_rules (mkP applySym applySig applyI).
+    Proof.
+      rewrite/check_rules/= andbT/check_rule.
+      rewrite [get_tm_hd _]/=.
+      cbn match.
+      rewrite !FmapE.fmapE eqxx .
+      rewrite [flatten_term _]/= [flatten_mode _]/= [flatten_sig _]/=.
+      rewrite/tm_is_det/get_tm_hd FmapE.fmapE.
+      rewrite orFb.
+      (* assume head *)
+      rewrite/assume_tm (@not_fnd _ _ _ (IV 2))//.
+      rewrite !FmapE.fmapE not_fnd//=.
+      (* check body, with F: exp -> pred, and V1: e *)
+      by rewrite/call_is_det /check_tm !FmapE.fmapE eqxx.
+    Qed.
+  End WrongApply.
+End Test.  
+    
 
 Lemma is_det_rename sP fv hd m:
   tm_is_det sP (rename fv hd m).2 =
@@ -49,20 +234,23 @@ Lemma fresh_has_cut sv xs m:
   has_cut_seq (fresh_atoms sv xs m).2 = has_cut_seq xs.
 Proof. by elim: xs sv => //= -[|c] xs IH sv; rewrite!push//=IH !push//. Qed.
 
-Lemma check_atom_fresh sP x sv m:
+(* Lemma check_atom_fresh sP x sv m:
   check_atom sP (fresh_atom sv x m).2 = check_atom sP x.
-Proof. by destruct x; rewrite //= !push/= is_det_rename. Qed.
+Proof. by destruct x; rewrite //= !push/= is_det_rename. Qed. *)
 
-Lemma all_check_atom_fresh sP xs sv m:
+(* Lemma all_check_atom_fresh sP xs sv m:
   all (check_atom sP) (fresh_atoms sv xs m).2 = all (check_atom sP) xs.
-Proof. by elim: xs sv => //=x xs IH sv; rewrite !push/= IH check_atom_fresh. Qed.
+Proof. by elim: xs sv => //=x xs IH sv; rewrite !push/= IH check_atom_fresh. Qed. *)
 
-Lemma check_atoms_fresh sP sv bo m:
-  check_atoms sP (fresh_atoms sv bo m).2 = check_atoms sP bo.
+(* Lemma check_atoms_fresh sP sV fv bo m d:
+  check_atoms sP sV (fresh_atoms fv bo m).2 d = check_atoms sP sV bo d.
 Proof.
-  elim: bo sv => //= -[|c] xs IH sv; rewrite !push//=IH//all_check_atom_fresh//.
+  elim: bo fv d => //= x xs IH fv d.
+  rewrite !push/=.
+  case: x => //= t.
+  rewrite !push/=.
   rewrite !push/= is_det_rename has_cut_seq_fresh//.
-Qed.
+Qed. *)
 
 Section check.
   Variable u : Unif.
@@ -80,14 +268,15 @@ Section check.
     end.
 
 
-  Fixpoint det_tree_seq sP L :=
+  Fixpoint det_tree_seq sP sV L :=
     match L with
     | [::] => true
-    | x :: xs => (check_atom sP x || has_cut_seq xs) && det_tree_seq sP xs
+    | x :: xs => (check_atom sP sV x || has_cut_seq xs) && det_tree_seq sP sV xs
     end.
 
-
   Definition nilA A := prune (success A) A == None.
+
+  Definition det_to_bool d := match d with Func => true | _ => false end.
 
   (** DOC:
     a tree is deterministic if it calls deterministic atoms. 
@@ -98,22 +287,22 @@ Section check.
     "((A, A') ; KO) , C" is det
     "(A ; B)" for any A and B is not det since nothing prevents the execution of B if A fails
   *)
-  Fixpoint det_tree (sP:sigT) A :=
+  Fixpoint det_tree (sP:sigT) sV A :=
     match A with
-    | TA a => check_atom sP a
+    | TA a => check_atom sP sV a
     | KO | OK => true
     | And A B0 B =>
-        det_tree sP B && 
+        det_tree sP sV B && 
         if nilA A
-        then det_tree sP A || has_cut B
+        then det_tree sP sV A || has_cut B
         else
           (* alternatives are mutually exclusive (only 1 alt can succeed) || B/B0 cuts them *)
-          (det_tree sP A || (has_cut B && has_cut_seq B0)) && (* has_cut B -> has_cut B0 in a valid tree ++ *)
-          det_tree_seq sP B0 (* if we backtrack in A, B0 must be det *)
-    | Or None _ B => det_tree sP B
+          (det_tree sP sV A || (has_cut B && has_cut_seq B0)) && (* has_cut B -> has_cut B0 in a valid tree ++ *)
+          det_tree_seq sP sV B0 (* if we backtrack in A, B0 must be det *)
+    | Or None _ B => det_tree sP sV B
     | Or (Some A) _ B =>
-        det_tree sP A && 
-        if has_cut A then det_tree sP B 
+        det_tree sP sV A && 
+        if has_cut A then det_tree sP sV B 
         else (B == KO) 
     end.
 
@@ -135,8 +324,8 @@ Section check.
     has_cut (big_and l) = has_cut_seq l.
   Proof. by case: l => >//; rewrite /=has_cut_big_and//. Qed.
 
-  Lemma det_tree_big_and sP L:
-    det_tree sP (big_and L) = det_tree_seq sP L.
+  Lemma det_tree_big_and sP sV L:
+    det_tree sP sV (big_and L) = det_tree_seq sP sV L.
   Proof.
     case: L => //= + L.
     elim: L => [|x xs IH][|c]//=; rewrite ?(orbF,andbT)//=IH;
@@ -144,8 +333,8 @@ Section check.
     by case: check_atom; case: det_tree_seq; case: has_cut_seq; rewrite//=andbF.
   Qed.
 
-  Lemma cut_followed_by_det_nfa_and {sP bo} :
-    check_atoms sP bo -> det_tree_seq sP bo.
+  Lemma cut_followed_by_det_nfa_and sP sV bo :
+    check_atoms sP sV bo -> det_tree_seq sP sV bo.
   Proof.
     elim: bo => //=.
     move=> [|t] /= l IH.
@@ -157,7 +346,7 @@ Section check.
   Lemma no_alt_cutl A: success A -> nilA (cutl A).
   Proof. by rewrite /nilA success_cut => ->; rewrite prune_cutl. Qed.
 
-  Lemma det_tree_cutl {sP A}: success A -> det_tree sP (cutl A).
+  Lemma det_tree_cutl {sP sV A}: success A -> det_tree sP sV (cutl A).
   Proof.
     elim_tree A => //=.
       by case: ifP => dA/= succ; rewrite !(HA,HB,eqxx,if_same)//=.
@@ -171,9 +360,10 @@ Section check.
   by simpl; rewrite !push.
   Qed.
 
-  Lemma check_rulesP p c fv s1:
+  (* Lemma check_rulesP p c fv s1:
     check_rules p ->
     tm_is_det p.(sig) c ->
+  (* TODO: should link sV with x.1 *)
     all (fun x => check_atoms p.(sig) x.2) (bc u p fv c s1).2.
   Proof.
     case: p => [rs s].
@@ -195,7 +385,7 @@ Section check.
     rewrite premises_fresh_rule/=.
     rewrite check_atoms_fresh.
     by move: TD c1; rewrite/check_rule/tm_is_det -tH C in_fnd => ->.
-  Qed.
+  Qed. *)
 
   Lemma deref_empty t:
     deref empty t = t.
@@ -234,11 +424,11 @@ Section check.
       has_cut (step u p sv s A).2.
   Proof. move/step_has_cut_help => /(_ p sv s)[]//->//. Qed.
 
-  Goal forall sP s, det_tree sP (Or (Some OK) s OK) == false.
+  Goal forall sP sV s, det_tree sP sV (Or (Some OK) s OK) == false.
   Proof. move=> ?? //=. Qed.
 
-  Lemma det_check_prune_succ {sP A} : 
-    det_tree sP A -> success A -> prune true A = None.
+  Lemma det_check_prune_succ {sP sV A} : 
+    det_tree sP sV A -> success A -> prune true A = None.
   Proof.
     elim: A => //=.
     - move=> A HA s B HB /andP[nA +]sA.
@@ -248,7 +438,7 @@ Section check.
     - move=> A HA B0 B HB /[!success_and]. 
       move=> /andP[dB +] /andP[sA sB].
       rewrite sA HB// success_has_cut// orbF.
-      rewrite -{1}[det_tree sP A]andbT -fun_if => /andP[? _].
+      rewrite -{1}[det_tree sP sV A]andbT -fun_if => /andP[? _].
       by rewrite HA.
   Qed.
 
@@ -281,8 +471,8 @@ Section check.
   Lemma prune_no_alt b A A' : prune b A  = Some A' -> success A = b -> nilA A = false.
   Proof. by rewrite /nilA=> + -> => ->. Qed.
 
-  Lemma det_check_prune {sP A R b}:
-    det_tree sP A -> prune b A = Some R -> det_tree sP R.
+  Lemma det_check_prune {sP sV A R b}:
+    det_tree sP sV A -> prune b A = Some R -> det_tree sP sV R.
   Proof.
     elim_tree A R b => /=.
     - by case: b => // _ [<-].
@@ -303,7 +493,7 @@ Section check.
           rewrite (HB B' b)//=.
           case cB: (has_cut B); first by rewrite (has_cut_prune cB nB).
           case cB': (has_cut B'); rewrite /= orbC //= ?orbT.
-          by rewrite -{1}[det_tree sP A]andbT -fun_if => /andP[-> //].
+          by rewrite -{1}[det_tree sP sV A]andbT -fun_if => /andP[-> //].
         case nA: prune => [A'|] //= + [<-/=].
         rewrite  has_cut_seq_has_cut_big_and det_tree_big_and (prune_no_alt nA)//.
         rewrite andbb=> /andP[+ ->]; rewrite andbT if_same /=.
@@ -319,10 +509,10 @@ Section check.
   Definition check_program pr := mut_excl u pr && check_rules pr.
   (*ENDSNIP: check_program *)
 
-  Lemma det_check_big_or_help s r0 rs:
-    all (fun x => check_atoms s x.2) (r0 :: rs) ->
+  Lemma det_check_big_or_help s sV r0 rs:
+    all (fun x => check_atoms s sV x.2) (r0 :: rs) ->
     all_but_last (fun x  => has_cut_seq x.2) (r0 :: rs) ->
-    det_tree s (big_or r0.2 rs).
+    det_tree s sV (big_or r0.2 rs).
   Proof.
     move=> /= => /andP[].
     elim: rs r0 => [|x xs IH] r0/= H; rewrite?push/=det_tree_big_and cut_followed_by_det_nfa_and//.
@@ -331,7 +521,8 @@ Section check.
     by apply: IH.
   Qed.
   
-  Lemma det_check_big_or pr c fv fv' r0 rs s1:
+  (* TODO: fixme *)
+  (* Lemma det_check_big_or pr c fv fv' r0 rs s1:
     check_program pr -> tm_is_det (sig pr) c -> 
     bc u pr fv c s1 = (fv', r0 :: rs) ->
     det_tree (sig pr) (big_or r0.2 rs).
@@ -353,7 +544,7 @@ Section check.
     rewrite S.
     rewrite AS/=.
     by apply/det_check_big_or_help.
-  Qed.
+  Qed. *)
 
   Fixpoint acyclic_sigmaT T :=
     match T with
@@ -373,7 +564,8 @@ Section check.
     move=> /andP[AA AB]; case: ifP; auto.
   Qed.
 
-  Lemma det_check_step pr sv s1 A r: 
+  (* TODO: fix me *)
+  (* Lemma det_check_step pr sv s1 A r: 
     check_program pr -> det_tree pr.(sig) A -> 
       step u pr sv s1 A = r ->
         det_tree pr.(sig) r.2.
@@ -403,10 +595,10 @@ Section check.
       case fA: (failed A).
         by rewrite /nilA /sA failed_step//= SA.
       case pA: (incomplete A).
-        rewrite/nilA incpl_prune//= => /andP[+ ->]/=.
+        rewrite/nilA incomplete_prune_id//= => /andP[+ ->]/=.
         by case/orP=> [/HA->/= | /[dup]/andP[-> ?] ->]; rewrite ?andbT ?orbT ?if_same.
       by have:= succF_failF_paF SA fA pA.
-  Qed.
+  Qed. *)
 
   (*SNIPT: is_det *)
   Definition is_det p s v t := 
@@ -516,35 +708,37 @@ Section check.
 
   (*SNIPT: det_check_tree *)
   Lemma det_check_tree: 
-    forall s v p t, check_program p -> det_tree p.(sig) t -> is_det p s v t.
+    forall s v p t fv, check_program p -> det_tree p.(sig) fv t -> is_det p s v t.
   (*ENDSNIPT: det_check_tree *)
   Proof.
     rewrite/is_det.
-    move=> s v p t H1 H2 r [b[v' R]].
+    move=> s v p t sV H1 H2 r [b[v' R]].
     elim_run R H1 H2.
     - rewrite (det_check_prune_succ H2 sA); eauto.
     - apply: IH => //=.
-        by apply: det_check_step eA.
+        (* by apply: det_check_step eA. *)
+        admit.
     - apply: IH => //.
       by apply/det_check_prune/nA.
-  Qed.
+  Admitted.
 
   (*SNIPT: det_check_call *)
   Theorem det_check_call:
-    forall p s t v, check_program p -> tm_is_det p.(sig) t -> is_det p s v (TA (call t)).
+    forall p s t v fv, 
+      check_program p -> call_is_det p.(sig) fv t -> is_det p s v (TA (call t)).
   (*ENDSNIPT: det_check_call *)
   Proof.
-    move=> /= p t s v cp td r H.
-    by apply/det_check_tree/H => //.
+    move=> /= p t s v fv cp td r H.
+    apply/det_check_tree/H => //=; eauto.
   Qed.
 
   (*SNIPT: det_check_calls *)
   Theorem det_check_calls:
-    forall p t v, check_program p -> tm_is_det p.(sig) t -> is_det p empty v (TA (call t)).
+    forall p t v fv, check_program p -> call_is_det p.(sig) fv t -> is_det p empty v (TA (call t)).
   (*ENDSNIPT: det_check_calls *)
   Proof.
-    move=> /= p t v cp td r H.
-    apply/det_check_tree/H => //.
+    move=> /= p t v cp fv td r H.
+    apply/det_check_tree/H => //; eauto.
   Qed.
 
 
@@ -583,6 +777,8 @@ Section check.
       move: H; apply:sub_all => -[hd bo].
       rewrite/tail_cut/=.
       rewrite/check_rule.
+      case: get_tm_hd => //= pred.
+      case: fndP => //= kp.
       case: tm_is_det => //=.
       elim: bo => //= x xs IH//=.
       destruct xs => //=[/eqP->|/[dup]{}/IH]//=->.
