theories/sig_lattice.v
@@ -1,0 +1,340 @@
+From det Require Import prelude.
+From mathcomp Require Import all_ssreflect.
+From det Require Import lang.
+
+  Definition maxD d1 d2 :=
+  match d1 with
+  | Pred => Pred
+  | _ => d2
+  end.
+
+Definition minD d1 d2 :=
+  match d1 with
+  | Func => Func
+  | Pred => d2
+  end.
+
+Lemma maxD_refl {r}: maxD r r = r.
+Proof. case: r => //. Qed.
+
+Lemma maxD_comm {l r}: maxD l r = maxD r l.
+Proof. case: l; case: r => //. Qed.
+
+Lemma minD_refl {r}: minD r r = r.
+Proof. case: r => //. Qed.
+
+Lemma minD_comm {l r}: minD l r = minD r l.
+Proof. case: l; case: r => //. Qed.
+
+Lemma maxD_assoc {x y z}: maxD x (maxD y z) = maxD (maxD x y) z.
+Proof. case: x => //=; case: y => //=; case: z => //. Qed.
+
+Lemma minD_assoc {x y z}: minD x (minD y z) = minD (minD x y) z.
+Proof. case: x => //=; case: y => //=; case: z => //. Qed.
+
+Definition negD x := match x with Pred => Func | Func => Pred end.  
+
+Fixpoint min_aux minD maxD s1 s2 : S :=
+  let is_min : bool := minD Pred Func == Func in
+  match s1, s2 with
+  | b Exp, b Exp => b Exp
+  | b(d D1), b(d D2) => b (d (minD D1 D2))
+  | arr input l1 r1, arr input l2 r2 => arr input (min_aux maxD minD l1 l2) (min_aux minD maxD r1 r2)
+  | arr output l1 r1, arr output l2 r2 => arr output (min_aux minD maxD l1 l2) (min_aux minD maxD r1 r2)
+
+  | b (d X), arr _ _ _ | b (d X), b Exp => 
+      if is_min then if X == Func then s1 else s2 else if X == Pred then s1 else s2
+  | arr _ _ _, b (d X) | b Exp, b (d X) => 
+      if is_min then if X == Pred then s1 else s2 else if X == Func then s1 else s2
+
+  | b Exp, arr _ _ _ | arr output _ _, arr input _ _ =>  if is_min then s1 else s2
+  | arr _ _ _, b Exp | arr input _ _, arr output _ _ => if ~~is_min then s1 else s2
+  end.
+
+Definition min := min_aux minD maxD.
+Definition max := min_aux maxD minD.
+
+Lemma min_refl {A}: min A A = A
+with max_refl {A}: max A A = A.
+Proof.
+  all: rewrite/min/max in min_refl max_refl *.
+  - by case d1: A => [[|[]]|[] bl br] //=; congr (arr _ _ _).
+  - by case d1: A => [[|[]]|[] bl br] //=; congr (arr _ _ _).
+Qed.
+
+Lemma min_comm {A B}: min A B = min B A
+with max_comm {A B}: max A B = max B A.
+Proof.
+  all: rewrite/min/max in min_comm max_comm *.
+  - by case d1: A => [[|[]]|[] bl br]; case d2: B => [[|[]]|[] cl cr] //=; congr(arr _ _ _).
+  - by case d1: A => [[|[]]|[] bl br]; case d2: B => [[|[]]|[] cl cr] //=; congr(arr _ _ _).
+Qed.
+
+Lemma min_assoc {A B C}: min A (min B C) = min (min A B) C
+with max_assoc {A B C}: max A (max B C) = max (max A B) C.
+Proof.
+  all: rewrite/max/min in min_assoc max_assoc *.
+  - case d1: A => [[|[]]|[] bl br]; case d2: B => [[|[]]|[] cl cr];
+    case d3: C => [[|[]]|[] dl dr]//=; f_equal; auto.
+  - case d1: A => [[|[]]|[] bl br]; case d2: B => [[|[]]|[] cl cr];
+    case d3: C => [[|[]]|[] dl dr]//=; f_equal; auto.
+Qed.
+
+Lemma min_assorb {A B}: min A (max A B) = A
+with max_assorb {A B}: max A (min A B) = A.
+Proof.
+  all: rewrite/max/min in min_assorb max_assorb *.
+  - case d1: A => [[|[]]|[] bl br]; case d2: B => [[|[]]|[] cl cr]//=; f_equal; auto; try by [apply min_refl | apply: max_refl].
+  - case d1: A => [[|[]]|[] bl br]; case d2: B => [[|[]]|[] cl cr]//=; f_equal; auto; try by [apply min_refl | apply: max_refl].
+Qed.
+
+Definition incl A B := (min A B == A).
+Definition not_incl A B := max A B == A.
+
+Lemma incl_refl {r}: incl r r.
+Proof. rewrite/incl min_refl//. Qed.
+
+Lemma incl_trans {A B C}: incl A B -> incl B C -> incl A C.
+Proof.
+  rewrite/incl.
+  move=> /eqP<-/eqP<-.
+  rewrite -!min_assoc min_refl//.
+Qed.
+
+Lemma min_incl {S1 S2 S3}: min S1 S2 = S3 -> (incl S3 S1).
+Proof. move=> <-; rewrite /incl min_comm min_assoc min_refl//. Qed.
+
+Lemma incl_min {S1 S2}: (incl S1 S2) -> min S1 S2 = S1.
+Proof. rewrite/incl => /eqP//. Qed.
+
+Lemma not_incl_incl {A B}: not_incl A B = incl B A.
+Proof. 
+  rewrite/not_incl/incl; do 2 case:eqP => //=.
+    move=> + H; rewrite-H.
+    rewrite max_comm min_assorb//.
+  move=> <-; rewrite min_comm max_assorb//.
+Qed.
+
+Lemma max2_incl {A B C D}:
+  max A B = C -> not_incl D A -> not_incl D B -> not_incl D C.
+Proof.
+  rewrite/not_incl.
+  move=> <- /eqP <- /eqP<-.
+  rewrite -2!max_assoc (@max_comm B) -max_assoc max_refl.
+  rewrite (@max_assoc A) max_refl -max_assoc//.
+Qed.
+
+Lemma min2_incl {A B C D}:
+  min A B = C -> incl D A -> incl D B -> incl D C.
+Proof.
+  rewrite/incl.
+  move=> <- /eqP <- /eqP<-.
+  rewrite -2!min_assoc (@min_comm B) -min_assoc min_refl.
+  rewrite (@min_assoc A) min_refl -min_assoc//.
+Qed.
+
+Lemma max2_incl1 {A B C D}:
+  max A B = C -> not_incl A D -> not_incl B D -> not_incl C D.
+Proof.
+  rewrite/not_incl.
+  move=> <- /eqP <- /eqP<-.
+  rewrite -!max_assoc max_refl//.
+Qed.
+
+Lemma min2_incl1 {A B C D}:
+  min A B = C -> incl A D -> incl B D -> incl C D.
+Proof.
+  rewrite/incl.
+  move=> <- /eqP <- /eqP<-.
+  rewrite -!min_assoc min_refl//.
+Qed.
+
+Lemma incl_inv {A B}: incl A B -> A = B \/ (incl B A) = false.
+Proof.
+  rewrite/incl => /eqP<-.
+  rewrite (@min_comm B) -min_assoc min_refl.
+  case:eqP; auto.
+Qed.
+
+Lemma not_incl_inv {A B}: not_incl A B -> A = B \/  (not_incl B A) = false.
+Proof.
+  rewrite/not_incl => /eqP<-.
+  rewrite (@max_comm B) -max_assoc max_refl.
+  case:eqP; auto.
+Qed.
+
+Fixpoint strong s :=
+  match s with
+  | b Exp => b Exp
+  | b(d _) => b(d Func)
+  | arr input l r => arr input (weak l) (strong r)
+  | arr output l r => arr output (strong l) (strong r)
+  end
+with weak s :=
+  match s with
+  | b Exp => b Exp
+  | b(d _) => b(d Pred) 
+  | arr input l r => arr input (strong l) (weak r)
+  | arr output l r => arr output (weak l) (weak r)
+  end.
+
+Section test.
+  Definition SMap := 
+    (arr input (arr input (b Exp) (arr output (b Exp) (b(d Func)))) (arr input (b Exp) (arr output (b Exp) (b(d Func))))).
+  Definition WMap := 
+    (arr input (arr input (b Exp) (arr output (b Exp) (b(d Func)))) (arr input (b Exp) (arr output (b Exp) (b(d Pred))))).
+  Goal incl SMap WMap. Proof. move=>//=. Qed.
+  Goal  (incl WMap SMap) = false. Proof. move=>//=. Qed.
+  Goal (weak SMap) == WMap. Proof. move=> //=. Qed.
+End test.
+
+Lemma min_strong {A}: min A (strong A) = (strong A)
+with max_weak {A}: max A (weak A) = (weak A).
+Proof.
+  all: rewrite/min/max in min_strong max_weak *.
+  - case: A => /=[[|[]]|[]s1 s2]//; rewrite ?min_strong ?max_weak//=.
+  - case: A => /=[[|[]]|[]s1 s2]//; rewrite ?min_strong ?max_weak//=.
+Qed.
+
+Lemma min_weak {A}: min A (weak A) = A
+with max_strong {A}: max A (strong A) = A.
+Proof.
+  all: rewrite/min/max in min_weak max_strong *.
+  - case: A => /=[[|[]]|[]s1 s2]//; rewrite /=?min_weak ?max_strong//=.
+  - case: A => /=[[|[]]|[]s1 s2]//; rewrite /=?min_weak ?max_strong//=.
+Qed.
+
+Lemma func_is_min {A}: incl (b (d Func)) A.
+Proof. rewrite/incl/=; case: A => //=[[]]//. Qed.
+
+Lemma pred_is_max {A}: incl A (b (d Pred)).
+Proof. rewrite/incl/=; case: A => //=[[|[]]|[]]//. Qed.
+
+Lemma weak_incl {A}: incl A (weak A).
+Proof. apply/eqP; apply: min_weak. Qed.
+
+Lemma max_predR {A}: max A (b (d Pred)) = (b (d Pred)).
+Proof. rewrite max_comm/max/=; case: A => [[]|]//. Qed.
+
+Lemma max_predL {A}: max (b (d Pred)) A = (b (d Pred)).
+Proof. case: A => [[|[]]|[]]//. Qed.
+
+Lemma max_funcR {A}: max A (b (d Func)) = A.
+Proof. rewrite max_comm/max/=; case: A => [[]|]//. Qed.
+
+Lemma max_funcL {A}: max (b (d Func)) A = A.
+Proof. case: A => [[|[]]|[]]//. Qed.
+
+Lemma min_funcR {A}: min A (b (d Func)) = (b (d Func)).
+Proof. rewrite min_comm/min/=; case: A => [[]|]//. Qed.
+
+Lemma min_funcL {A}: min (b (d Func)) A = (b (d Func)).
+Proof. case: A => [[|[]]|[]]//. Qed.
+
+Lemma strong_incl {A}: incl (strong A) A.
+Proof. apply: min_incl min_strong. Qed.
+
+Lemma weak2 {A}: weak (weak A) = weak A
+with strong2 {A}: strong (strong A) = strong A.
+Proof. all: case: A => -[]//=??; rewrite?weak2?strong2//. Qed.
+
+Lemma weak_strong {A B}: weak A = weak B -> strong A = strong B
+with strong_weak {A B}: strong A = strong B -> weak A = weak B.
+Proof.
+  - case: A => [[|[]]|[] l1 r1]; case: B => [[]|[]l2 r2]//= [H1 H2]; f_equal; auto.
+  - case: A => [[|[]]|[] l1 r1]; case: B => [[]|[]l2 r2]//= [H1 H2]; f_equal; auto.
+Qed.
+
+Lemma min_arr s t s' t' m : min (arr m s' t') (arr m s t)  = arr m (if m == input then max s' s else min s' s) (min t' t). by case: m. Qed.
+Lemma max_arr s t s' t' m : max (arr m s' t') (arr m s t)  = arr m (if m == input then min s' s else max s' s) (max t' t). by case: m. Qed.
+
+Lemma incl_arr s t s' t' m :
+  incl (arr m s' t') (arr m s t) = (if m == input then incl s s' else incl s' s) && incl t' t.
+Proof.
+  rewrite /incl min_arr; case: m => /=; symmetry; (repeat case: eqP); try by [|congruence].
+  - by move=> + E F; rewrite E -F min_comm max_assorb.
+  - by move=> [] <- ??; rewrite max_comm min_assorb.
+Qed.
+
+Lemma min_weakr s t : min (min s t) (weak t) = min s t
+with max_strongr s t : max (max s t) (strong t) = max s t.
+Proof.
+  all: rewrite/min/max in min_weakr max_strongr *.
+  - case: s => [[|[]]|[] f1 a1]; case: t => [[|[]]|[] f2 a2]//=; f_equal; auto;
+    try by [apply max_strong|apply: min_weak].
+  - case: s => [[|[]]|[] f1 a1]; case: t => [[|[]]|[] f2 a2]//=; f_equal; auto;
+    try by [apply max_strong|apply: min_weak].
+Qed.
+
+Lemma incl_weakr s t : incl s t -> incl s (weak t).
+Proof. move=> /eqP <-; apply/eqP/min_weakr. Qed.
+
+Lemma incl_weakl t: incl (weak t) t -> weak t = t.
+Proof. by move=> /eqP; rewrite min_comm min_weak. Qed.
+
+
+Lemma min_abb a b: min (min a b) b = min a b.
+Proof. rewrite -min_assoc min_refl//. Qed.
+
+Lemma max_abb a b: max (max a b) b = max a b.
+Proof. rewrite -max_assoc max_refl//. Qed.
+
+Lemma inclL_max A B C: incl A C -> incl B C -> incl (max A B) C
+with inclR_min A B C: incl C A -> incl C B -> incl C (min A B).
+Proof.
+    case: A => [[|[]]|[] f a]; case: B => [[|[]]|[] f1 a1]; 
+    case: C => [[|[]]|[] f2 a2]//=; rewrite ?pred_is_max//=?max_arr/=?incl_arr//=; cycle 1;
+    [|move=> /andP[H1 H2] /andP[H3 H4]; apply/andP; split; auto..];
+    rewrite/incl/min/=//.
+  move=> /eqP<-/eqP<-; apply/eqP.
+  rewrite -!min_assoc.
+  by rewrite (@min_assoc A B) min_refl.
+Qed.
+
+Lemma incl2_max A B C D: incl A C -> incl B D -> incl (max A B) (max C D)
+with incl2_min A B C D: incl A C -> incl B D -> incl (min A B) (min C D).
+Proof.
+  move=> H1 H2; apply: inclL_max.
+  - move: H1; rewrite /incl => /eqP <-.
+    rewrite -min_assoc min_assorb//.
+  - move: H2; rewrite /incl => /eqP <-.
+    rewrite -min_assoc max_comm min_assorb//.
+  move=> H1 H2; apply: inclR_min.
+  - move: H1; rewrite /incl => /eqP <-.
+    rewrite min_comm min_assoc (@min_comm C) -(@min_assoc A C C) min_refl//.
+  - move: H2; rewrite /incl => /eqP <-.
+    by rewrite -!min_assoc min_refl.
+Qed.
+
+Lemma inclL_min A B C: incl A C -> incl (min A B) C
+with inclR_max A B C: incl A C -> incl A (max B C).
+Proof.
+    move=>/eqP<-; apply/eqP.
+    rewrite min_comm min_assoc.
+    by rewrite (@min_comm A) min_assoc min_refl.
+  case: A => [[|[]]|[] f a]; case: C => [[|[]]|[] f2 a2]//=;
+  rewrite ?max_predR ?pred_is_max ?func_is_min//=;
+  case: B => [[|[]]|[] f3 a3]/=;
+  rewrite ?max_arr/=?max_predL?max_funcL ?pred_is_max?incl_arr//=; cycle 2.
+  - by move=> /andP[]/inclR_max->/inclR_max->.
+  - by rewrite min_comm; move=> /andP[/inclL_min->/inclR_max->]//.
+  - rewrite/max/={3}/incl/=/min/=//.
+Qed.
+
+Lemma eq_incl x y : (incl x y && incl y x) = (x == y).
+Proof.
+  apply/andP/eqP => [[]|-> //]; rewrite?incl_refl//.
+  by move=> /eqP<-/eqP<-; rewrite min_assoc min_refl (@min_comm x) min_assoc min_refl.
+Qed.
+
+Lemma min_strong2 {A B}: strong (min (strong A) (strong B)) = (min (strong A) (strong B))
+with max_weak2 {A B}: weak (max (weak A) (weak B)) = (max (weak A) (weak B)).
+Proof.
+  all: rewrite/min/max in min_strong2 max_weak2 *.
+  - case: A => /=[[|[]]|[]s1 s2]//; case: B => /=[[|[]]|[]s3 s4]//=; rewrite ?strong2//; f_equal; auto.
+  - case: A => /=[[|[]]|[]s1 s2]//; case: B => /=[[|[]]|[]s3 s4]//=; rewrite ?strong2//?weak2; f_equal; auto.
+Qed.
+
+Global Hint Resolve incl_refl : core.
+Global Hint Resolve minD_refl : core.
+
