theories/tree_vars.v
@@ -43,7 +43,7 @@ Section vars_tree.
     move => H1 H2.
     rewrite/bc/=.
     case: ifP => //= _.
-    case X: get_tm_hd => [c'|]//=.
+    case X: get_tm_hd => //[pred].
     case: fndP => /=hp; last by move=> [<-].
     rewrite !push.
     case FR: fresh_rules => [fF RF]/=.
